examples/sll_init.v
@@ -9,11 +9,11 @@ Require Import core.
 
 Inductive sll (x : ptr) (s : seq nat) (h : heap) : Prop :=
 | sll1 of x == 0 of
-  s = nil /\ h = empty
+  perm_eq (s) (nil) /\ h = empty
 | sll2 of ~~ (x == 0) of
-  exists v s1 nxt,
-  exists h_sll526,
-  s = [:: v] ++ s1 /\ h = x :-> v \+ x .+ 1 :-> nxt \+ h_sll526 /\ sll nxt s1 h_sll526.
+  exists (v : nat) (s1 : seq nat) nxt,
+  exists h_sll_nxts1_537,
+  perm_eq (s) ([:: v] ++ s1) /\ h = x :-> v \+ x .+ 1 :-> nxt \+ h_sll_nxts1_537 /\ sll nxt s1 h_sll_nxts1_537.
 
 Definition sll_init_type :=
   forall (vprogs : ptr * nat),
@@ -22,14 +22,14 @@ Definition sll_init_type :=
     fun h =>
       let: (x, v) := vprogs in
       let: (s) := vghosts in
-      exists h_sll527,
-      h = h_sll527 /\ sll x s h_sll527,
+      exists h_sll_xs_538,
+      h = h_sll_xs_538 /\ sll x s h_sll_xs_538,
     [vfun (_: unit) h =>
       let: (x, v) := vprogs in
       let: (s) := vghosts in
       exists s1,
-      exists h_sll528,
-      {subset s1 <= [:: v]} /\ h = h_sll528 /\ sll x s1 h_sll528
+      exists h_sll_xs1_539,
+      {subset s1 <= [:: v]} /\ h = h_sll_xs1_539 /\ sll x s1 h_sll_xs1_539
     ]).
 Program Definition sll_init : sll_init_type :=
   Fix (fun (sll_init : sll_init_type) vprogs =>
@@ -48,51 +48,51 @@ Obligation Tactic := intro; move=>[x v]; ssl_program_simpl.
 Next Obligation.
 ssl_ghostelim_pre.
 move=>s.
-move=>[h_sll527].
+ex_elim h_sll_xs_538.
 move=>[sigma_self].
-rewrite->sigma_self in *.
-move=>H_sll527.
+subst.
+move=>H_sll_xs_538.
 ssl_ghostelim_post.
 ssl_open.
-ssl_open_post H_sll527.
-move=>[phi_sll527].
-move=>[sigma_sll527].
-rewrite->sigma_sll527 in *.
+ssl_open_post H_sll_xs_538.
+move=>[phi_sll_xs_538].
+move=>[sigma_sll_xs_538].
+subst.
 ssl_emp;
 exists (nil);
 exists (empty);
 sslauto.
 unfold_constructor 1;
 sslauto.
-ssl_open_post H_sll527.
-move=>[vx2] [s1x] [nxtx2].
-move=>[h_sll526x].
-move=>[phi_sll527].
-move=>[sigma_sll527].
-rewrite->sigma_sll527 in *.
-move=>H_sll526x.
+ssl_open_post H_sll_xs_538.
+ex_elim vx2 s1x nxtx2.
+ex_elim h_sll_nxtx2s1x_537x.
+move=>[phi_sll_xs_538].
+move=>[sigma_sll_xs_538].
+subst.
+move=>H_sll_nxtx2s1x_537x.
 ssl_read.
-ssl_call_pre (h_sll526x).
+ssl_call_pre (h_sll_nxtx2s1x_537x).
 ssl_call (s1x).
-exists (h_sll526x);
+exists (h_sll_nxtx2s1x_537x);
 sslauto.
-move=>h_call6.
-move=>[s11].
-move=>[h_sll5281].
-move=>[phi_call6].
-move=>[sigma_call6].
-rewrite->sigma_call6 in *.
-move=>H_sll5281.
+move=>h_call10.
+ex_elim s11.
+ex_elim h_sll_nxtx2s11_5391.
+move=>[phi_call10].
+move=>[sigma_call10].
+subst.
+move=>H_sll_nxtx2s11_5391.
 store_valid.
-ssl_write.
+ssl_write x.
 ssl_write_post x.
 ssl_emp;
 exists ([:: v] ++ s11);
-exists (x :-> v \+ x .+ 1 :-> nxtx2 \+ h_sll5281);
+exists (x :-> v \+ x .+ 1 :-> nxtx2 \+ h_sll_nxtx2s11_5391);
 sslauto.
 unfold_constructor 2;
 exists (v), (s11), (nxtx2);
-exists (h_sll5281);
+exists (h_sll_nxtx2s11_5391);
 sslauto.
 
 Qed.
