examples/tree_free.v
@@ -9,28 +9,28 @@ Require Import core.
 
 Inductive tree (x : ptr) (s : seq nat) (h : heap) : Prop :=
 | tree1 of x == 0 of
-  s = nil /\ h = empty
+  perm_eq (s) (nil) /\ h = empty
 | tree2 of ~~ (x == 0) of
-  exists v s1 s2 l r,
-  exists h_tree519 h_tree520,
-  s = [:: v] ++ s1 ++ s2 /\ h = x :-> v \+ x .+ 1 :-> l \+ x .+ 2 :-> r \+ h_tree519 \+ h_tree520 /\ tree l s1 h_tree519 /\ tree r s2 h_tree520.
+  exists (v : nat) (s1 : seq nat) (s2 : seq nat) l r,
+  exists h_tree_ls1_523 h_tree_rs2_524,
+  perm_eq (s) ([:: v] ++ s1 ++ s2) /\ h = x :-> v \+ x .+ 1 :-> l \+ x .+ 2 :-> r \+ h_tree_ls1_523 \+ h_tree_rs2_524 /\ tree l s1 h_tree_ls1_523 /\ tree r s2 h_tree_rs2_524.
 
-Definition treefree_type :=
+Definition tree_free_type :=
   forall (vprogs : ptr),
   {(vghosts : seq nat)},
   STsep (
     fun h =>
       let: (x) := vprogs in
       let: (s) := vghosts in
-      exists h_tree521,
-      h = h_tree521 /\ tree x s h_tree521,
+      exists h_tree_xs_525,
+      h = h_tree_xs_525 /\ tree x s h_tree_xs_525,
     [vfun (_: unit) h =>
       let: (x) := vprogs in
       let: (s) := vghosts in
       h = empty
     ]).
-Program Definition treefree : treefree_type :=
-  Fix (fun (treefree : treefree_type) vprogs =>
+Program Definition tree_free : tree_free_type :=
+  Fix (fun (tree_free : tree_free_type) vprogs =>
     let: (x) := vprogs in
     Do (
       if x == 0
@@ -39,8 +39,8 @@ Program Definition treefree : treefree_type :=
       else
         lx2 <-- @read ptr (x .+ 1);
         rx2 <-- @read ptr (x .+ 2);
-        treefree (lx2);;
-        treefree (rx2);;
+        tree_free (lx2);;
+        tree_free (rx2);;
         dealloc x;;
        dealloc (x .+ 1);;
        dealloc (x .+ 2);;
@@ -50,42 +50,42 @@ Obligation Tactic := intro; move=>x; ssl_program_simpl.
 Next Obligation.
 ssl_ghostelim_pre.
 move=>s.
-move=>[h_tree521].
+ex_elim h_tree_xs_525.
 move=>[sigma_self].
-rewrite->sigma_self in *.
-move=>H_tree521.
+subst.
+move=>H_tree_xs_525.
 ssl_ghostelim_post.
 ssl_open.
-ssl_open_post H_tree521.
-move=>[phi_tree521].
-move=>[sigma_tree521].
-rewrite->sigma_tree521 in *.
+ssl_open_post H_tree_xs_525.
+move=>[phi_tree_xs_525].
+move=>[sigma_tree_xs_525].
+subst.
 ssl_emp;
 sslauto.
-ssl_open_post H_tree521.
-move=>[vx2] [s1x] [s2x] [lx2] [rx2].
-move=>[h_tree519x] [h_tree520x].
-move=>[phi_tree521].
-move=>[sigma_tree521].
-rewrite->sigma_tree521 in *.
-move=>[H_tree519x H_tree520x].
+ssl_open_post H_tree_xs_525.
+ex_elim vx2 s1x s2x lx2 rx2.
+ex_elim h_tree_lx2s1x_523x h_tree_rx2s2x_524x.
+move=>[phi_tree_xs_525].
+move=>[sigma_tree_xs_525].
+subst.
+move=>[H_tree_lx2s1x_523x H_tree_rx2s2x_524x].
 ssl_read.
 ssl_read.
-ssl_call_pre (h_tree519x).
+ssl_call_pre (h_tree_lx2s1x_523x).
 ssl_call (s1x).
-exists (h_tree519x);
+exists (h_tree_lx2s1x_523x);
 sslauto.
-move=>h_call3.
-move=>[sigma_call3].
-rewrite->sigma_call3 in *.
+move=>h_call5.
+move=>[sigma_call5].
+subst.
 store_valid.
-ssl_call_pre (h_tree520x).
+ssl_call_pre (h_tree_rx2s2x_524x).
 ssl_call (s2x).
-exists (h_tree520x);
+exists (h_tree_rx2s2x_524x);
 sslauto.
-move=>h_call4.
-move=>[sigma_call4].
-rewrite->sigma_call4 in *.
+move=>h_call6.
+move=>[sigma_call6].
+subst.
 store_valid.
 ssl_dealloc.
 ssl_dealloc.
