examples/dll_dupleton.v
@@ -1,0 +1,88 @@
+From mathcomp
+Require Import ssreflect ssrbool ssrnat eqtype seq ssrfun.
+From fcsl
+Require Import prelude pred pcm unionmap heap.
+From HTT
+Require Import stmod stsep stlog stlogR.
+From SSL
+Require Import core.
+
+Inductive dll (x : ptr) (z : ptr) (s : seq nat) (h : heap) : Prop :=
+| dll1 of x == 0 of
+  perm_eq (s) (nil) /\ h = empty
+| dll2 of ~~ (x == 0) of
+  exists (v : nat) (s1 : seq nat) w,
+  exists h_dll_wxs1_540,
+  perm_eq (s) ([:: v] ++ s1) /\ h = x :-> v \+ x .+ 1 :-> w \+ x .+ 2 :-> z \+ h_dll_wxs1_540 /\ dll w x s1 h_dll_wxs1_540.
+
+Inductive sll (x : ptr) (s : seq nat) (h : heap) : Prop :=
+| sll1 of x == 0 of
+  perm_eq (s) (nil) /\ h = empty
+| sll2 of ~~ (x == 0) of
+  exists (v : nat) (s1 : seq nat) nxt,
+  exists h_sll_nxts1_541,
+  perm_eq (s) ([:: v] ++ s1) /\ h = x :-> v \+ x .+ 1 :-> nxt \+ h_sll_nxts1_541 /\ sll nxt s1 h_sll_nxts1_541.
+
+Definition dll_dupleton_type :=
+  forall (vprogs : nat * nat * ptr),
+  {(vghosts : ptr)},
+  STsep (
+    fun h =>
+      let: (x, y, r) := vprogs in
+      let: (a) := vghosts in
+      h = r :-> a,
+    [vfun (_: unit) h =>
+      let: (x, y, r) := vprogs in
+      let: (a) := vghosts in
+      exists (elems : seq nat) z,
+      exists h_dll_zelems_542,
+      perm_eq (elems) ([:: x; y]) /\ h = r :-> z \+ h_dll_zelems_542 /\ dll z 0 elems h_dll_zelems_542
+    ]).
+Program Definition dll_dupleton : dll_dupleton_type :=
+  Fix (fun (dll_dupleton : dll_dupleton_type) vprogs =>
+    let: (x, y, r) := vprogs in
+    Do (
+      z2 <-- allocb null 3;
+      wz2 <-- allocb null 3;
+      r ::= z2;;
+      (z2 .+ 1) ::= wz2;;
+      (z2 .+ 2) ::= null;;
+      (wz2 .+ 1) ::= null;;
+      (wz2 .+ 2) ::= z2;;
+      z2 ::= y;;
+      wz2 ::= x;;
+      ret tt
+    )).
+Obligation Tactic := intro; move=>[[x y] r]; ssl_program_simpl.
+Next Obligation.
+ssl_ghostelim_pre.
+move=>a2.
+move=>[sigma_self].
+subst.
+ssl_ghostelim_post.
+ssl_alloc z2.
+ssl_alloc wz2.
+ssl_write r.
+ssl_write_post r.
+ssl_write (z2 .+ 1).
+ssl_write_post (z2 .+ 1).
+ssl_write (z2 .+ 2).
+ssl_write_post (z2 .+ 2).
+ssl_write (wz2 .+ 1).
+ssl_write_post (wz2 .+ 1).
+ssl_write (wz2 .+ 2).
+ssl_write_post (wz2 .+ 2).
+ssl_write z2.
+ssl_write_post z2.
+ssl_write wz2.
+ssl_write_post wz2.
+ssl_emp;
+exists ([:: x; y]), (z2);
+exists (0 :-> y \+ 0 .+ 1 :-> wz2 \+ 0 .+ 2 :-> null \+ h_dll_wz2x_540z);
+sslauto.
+unfold_constructor 2;
+exists (y), ([:: x] ++ nil), (wz2);
+exists (h_dll_wz2x_540z);
+sslauto.
+
+Qed.
