examples/dll_singleton.v
@@ -1,0 +1,79 @@
+From mathcomp
+Require Import ssreflect ssrbool ssrnat eqtype seq ssrfun.
+From fcsl
+Require Import prelude pred pcm unionmap heap.
+From HTT
+Require Import stmod stsep stlog stlogR.
+From SSL
+Require Import core.
+
+Inductive dll (x : ptr) (z : ptr) (s : seq nat) (h : heap) : Prop :=
+| dll1 of x == 0 of
+  perm_eq (s) (nil) /\ h = empty
+| dll2 of ~~ (x == 0) of
+  exists (v : nat) (s1 : seq nat) w,
+  exists h_dll_wxs1_543,
+  perm_eq (s) ([:: v] ++ s1) /\ h = x :-> v \+ x .+ 1 :-> w \+ x .+ 2 :-> z \+ h_dll_wxs1_543 /\ dll w x s1 h_dll_wxs1_543.
+
+Inductive sll (x : ptr) (s : seq nat) (h : heap) : Prop :=
+| sll1 of x == 0 of
+  perm_eq (s) (nil) /\ h = empty
+| sll2 of ~~ (x == 0) of
+  exists (v : nat) (s1 : seq nat) nxt,
+  exists h_sll_nxts1_544,
+  perm_eq (s) ([:: v] ++ s1) /\ h = x :-> v \+ x .+ 1 :-> nxt \+ h_sll_nxts1_544 /\ sll nxt s1 h_sll_nxts1_544.
+
+Definition dll_singleton_type :=
+  forall (vprogs : nat * ptr),
+  {(vghosts : ptr)},
+  STsep (
+    fun h =>
+      let: (x, r) := vprogs in
+      let: (a) := vghosts in
+      h = r :-> a,
+    [vfun (_: unit) h =>
+      let: (x, r) := vprogs in
+      let: (a) := vghosts in
+      exists (elems : seq nat) y,
+      exists h_dll_yelems_545,
+      perm_eq (elems) ([:: x]) /\ h = r :-> y \+ h_dll_yelems_545 /\ dll y 0 elems h_dll_yelems_545
+    ]).
+Program Definition dll_singleton : dll_singleton_type :=
+  Fix (fun (dll_singleton : dll_singleton_type) vprogs =>
+    let: (x, r) := vprogs in
+    Do (
+      y2 <-- allocb null 3;
+      r ::= y2;;
+      (y2 .+ 1) ::= null;;
+      (y2 .+ 2) ::= null;;
+      y2 ::= x;;
+      ret tt
+    )).
+Obligation Tactic := intro; move=>[x r]; ssl_program_simpl.
+Next Obligation.
+ssl_ghostelim_pre.
+move=>a2.
+move=>[sigma_self].
+subst.
+ssl_ghostelim_post.
+ssl_alloc y2.
+ssl_write r.
+ssl_write_post r.
+ssl_write (y2 .+ 1).
+ssl_write_post (y2 .+ 1).
+ssl_write (y2 .+ 2).
+ssl_write_post (y2 .+ 2).
+ssl_write y2.
+ssl_write_post y2.
+ssl_emp;
+exists ([:: x]), (y2);
+exists (y2 :-> x \+ y2 .+ 1 :-> null \+ y2 .+ 2 :-> null);
+sslauto.
+unfold_constructor 2;
+exists (x), (nil), (0);
+exists (empty);
+sslauto.
+unfold_constructor 1;
+sslauto.
+
+Qed.
