examples/sll_append.v
@@ -1,0 +1,121 @@
+From mathcomp
+Require Import ssreflect ssrbool ssrnat eqtype seq ssrfun finset.
+From fcsl
+Require Import prelude pred pcm unionmap heap.
+From HTT
+Require Import stmod stsep stlog stlogR.
+From SSL
+Require Import core.
+
+Inductive sll (x : ptr) (s : seq nat) (h : heap) : Prop :=
+| sll1 of x == 0 of
+  perm_eq (s) (nil) /\ h = empty
+| sll2 of ~~ (x == 0) of
+  exists (v : nat) (s1 : seq nat) nxt,
+  exists h_sll528,
+    perm_eq s ([:: v] ++ s1) /\ h = x :-> v \+ x .+ 1 :-> nxt \+ h_sll528 /\ sll nxt s1 h_sll528.
+
+Lemma sll_perm_eq x s h s1 :
+  perm_eq s s1 -> sll x s h -> sll x s1 h.
+Proof.
+move=>Heq Hsll; sslauto.
+case: Hsll=>cond.
+move=>[Heq1 ->].
+constructor 1=>//=; sslauto.
+move=>[v] [s2] [nxt] [h'].
+move=>[Heq1 [-> Hssl]].
+constructor 2=>//=.
+exists v, s2, nxt, h'.
+sslauto.
+rewrite perm_sym in Heq.
+apply: (perm_trans Heq Heq1).
+Qed.
+
+
+Definition sll_append_type :=
+  forall (vprogs : ptr * ptr),
+  {(vghosts : seq nat * seq nat * ptr)},
+  STsep (
+    fun h =>
+      let: (x1, r) := vprogs in
+      let: (s1, s2, x2) := vghosts in
+      exists h_sll529 h_sll530,
+      h = r :-> x2 \+ h_sll529 \+ h_sll530 /\ sll x1 s1 h_sll529 /\ sll x2 s2 h_sll530,
+    [vfun (_: unit) h =>
+      let: (x1, r) := vprogs in
+      let: (s1, s2, x2) := vghosts in
+      exists (s : seq nat) y,
+      exists h_sll531,
+      perm_eq s (s1 ++ s2) /\ h = r :-> y \+ h_sll531 /\ sll y s h_sll531
+    ]).
+Program Definition sll_append : sll_append_type :=
+  Fix (fun (sll_append : sll_append_type) vprogs =>
+    let: (x1, r) := vprogs in
+    Do (
+      if x1 == 0
+      then
+        ret tt
+      else
+        nxtx12 <-- @read ptr (x1 .+ 1);
+        sll_append (nxtx12, r);;
+        y12 <-- @read ptr r;
+        (x1 .+ 1) ::= y12;;
+        r ::= x1;;
+        ret tt
+    )).
+Obligation Tactic := intro; move=>[x1 r]; ssl_program_simpl.
+Next Obligation.
+ssl_ghostelim_pre.
+move=>[[s1 s2] x22].
+move=>[h_sll529] [h_sll530].
+move=>[sigma_self].
+subst.
+move=>[H_sll529 H_sll530].
+ssl_ghostelim_post.
+ssl_open.
+ssl_open_post H_sll529.
+move=>[phi_sll529].
+move=>[sigma_sll529].
+subst.
+ssl_emp;
+exists (nil ++ s2), (x22);
+exists (h_sll530);
+sslauto.
+ssl_open_post H_sll529.
+move=>[vx12] [s1x1] [nxtx12].
+move=>[h_sll528x1].
+move=>[phi_sll529].
+move=>[sigma_sll529].
+subst.
+move=>H_sll528x1.
+ssl_read.
+ssl_call_pre (r :-> x22 \+ h_sll528x1 \+ h_sll530).
+ssl_call (s1x1, s2, x22).
+exists (h_sll528x1);
+exists (h_sll530);
+sslauto.
+move=>h_call8.
+move=>[s3] [y12].
+move=>[h_sll5311].
+move=>[phi_call8].
+move=>[sigma_call8].
+subst.
+move=>H_sll5311.
+store_valid.
+ssl_read.
+ssl_write (x1 .+ 1).
+ssl_write_post (x1 .+ 1).
+ssl_write r.
+ssl_write_post r.
+ssl_emp;
+exists ([:: vx12] ++ s1x1 ++ s2), (x1);
+exists (x1 :-> vx12 \+ x1 .+ 1 :-> y12 \+ h_sll5311);
+sslauto.
+rewrite -cat_cons perm_cat2r perm_sym=>//=.
+unfold_constructor 2;
+exists (vx12), (s1x1 ++ s2), (y12);
+exists (h_sll5311);
+sslauto.
+apply: (sll_perm_eq _ s3)=>//=.
+Qed.
+
