examples/sll_dupleton.v
@@ -1,0 +1,80 @@
+From mathcomp
+Require Import ssreflect ssrbool ssrnat eqtype seq ssrfun.
+From fcsl
+Require Import prelude pred pcm unionmap heap.
+From HTT
+Require Import stmod stsep stlog stlogR.
+From SSL
+Require Import core.
+
+Inductive sll (x : ptr) (s : seq nat) (h : heap) : Prop :=
+| sll1 of x == 0 of
+  s = nil /\ h = empty
+| sll2 of ~~ (x == 0) of
+  exists v s1 nxt,
+  exists h_sll513,
+  s = [:: v] ++ s1 /\ h = x :-> v \+ x .+ 1 :-> nxt \+ h_sll513 /\ sll nxt s1 h_sll513.
+
+Definition sll_dupleton_type :=
+  forall (vprogs : nat * nat * ptr),
+  {(vghosts : ptr)},
+  STsep (
+    fun h =>
+      let: (x, y, r) := vprogs in
+      let: (a) := vghosts in
+      h = r :-> a,
+    [vfun (_: unit) h =>
+      let: (x, y, r) := vprogs in
+      let: (a) := vghosts in
+      exists (elems : seq nat) z,
+      exists h_sll514,
+      elems = [:: x; y] /\ h = r :-> z \+ h_sll514 /\ sll z elems h_sll514
+    ]).
+Program Definition sll_dupleton : sll_dupleton_type :=
+  Fix (fun (sll_dupleton : sll_dupleton_type) vprogs =>
+    let: (x, y, r) := vprogs in
+    Do (
+      z2 <-- allocb null 2;
+      nxtz2 <-- allocb null 2;
+      r ::= z2;;
+      (z2 .+ 1) ::= nxtz2;;
+      (nxtz2 .+ 1) ::= null;;
+      z2 ::= x;;
+      nxtz2 ::= y;;
+      ret tt
+    )).
+Obligation Tactic := intro; move=>[[x y] r]; ssl_program_simpl.
+Next Obligation.
+ssl_ghostelim_pre.
+move=>a2.
+move=>[sigma_self].
+subst.
+ssl_ghostelim_post.
+ssl_alloc z2.
+ssl_alloc nxtz2.
+ssl_write r.
+ssl_write_post r.
+ssl_write (z2 .+ 1).
+ssl_write_post (z2 .+ 1).
+ssl_write (nxtz2 .+ 1).
+ssl_write_post (nxtz2 .+ 1).
+ssl_write z2.
+ssl_write_post z2.
+ssl_write nxtz2.
+ssl_write_post nxtz2.
+ssl_emp;
+exists ([:: x; y]), (z2);
+exists (z2 :-> x \+ z2 .+ 1 :-> nxtz2 \+ nxtz2 :-> y \+ nxtz2 .+ 1 :-> null);
+sslauto.
+unfold_constructor 2;
+exists (x), ([:: y] ++ nil), (nxtz2);
+exists (nxtz2 :-> y \+ nxtz2 .+ 1 :-> null);
+sslauto.
+unfold_constructor 2;
+exists (y), (nil), (0);
+exists (empty);
+sslauto.
+unfold_constructor 1;
+sslauto.
+
+Qed.
