examples/tree_copy.v
@@ -1,0 +1,144 @@
+From mathcomp
+Require Import ssreflect ssrbool ssrnat eqtype seq ssrfun.
+From fcsl
+Require Import prelude pred pcm unionmap heap.
+From HTT
+Require Import stmod stsep stlog stlogR.
+From SSL
+Require Import core.
+
+Inductive tree (x : ptr) (s : seq nat) (h : heap) : Prop :=
+| tree1 of x == 0 of
+  perm_eq (s) (nil) /\ h = empty
+| tree2 of ~~ (x == 0) of
+  exists (v : nat) (s1 : seq nat) (s2 : seq nat) l r,
+  exists h_tree_ls1_521 h_tree_rs2_522,
+  perm_eq (s) ([:: v] ++ s1 ++ s2) /\ h = x :-> v \+ x .+ 1 :-> l \+ x .+ 2 :-> r \+ h_tree_ls1_521 \+ h_tree_rs2_522 /\ tree l s1 h_tree_ls1_521 /\ tree r s2 h_tree_rs2_522.
+
+Definition tree_copy_type :=
+  forall (vprogs : ptr),
+  {(vghosts : ptr * seq nat)},
+  STsep (
+    fun h =>
+      let: (r) := vprogs in
+      let: (x, s) := vghosts in
+      exists h_tree_xs_a,
+      h = r :-> x \+ h_tree_xs_a /\ tree x s h_tree_xs_a,
+    [vfun (_: unit) h =>
+      let: (r) := vprogs in
+      let: (x, s) := vghosts in
+      exists y,
+      exists h_tree_xs_a h_tree_ys_a,
+      h = r :-> y \+ h_tree_xs_a \+ h_tree_ys_a /\ tree x s h_tree_xs_a /\ tree y s h_tree_ys_a
+    ]).
+Program Definition tree_copy : tree_copy_type :=
+  Fix (fun (tree_copy : tree_copy_type) vprogs =>
+    let: (r) := vprogs in
+    Do (
+      x2 <-- @read ptr r;
+      if x2 == 0
+      then
+        ret tt
+      else
+        vx22 <-- @read nat x2;
+        lx22 <-- @read ptr (x2 .+ 1);
+        rx22 <-- @read ptr (x2 .+ 2);
+        r ::= lx22;;
+        tree_copy (r);;
+        y12 <-- @read ptr r;
+        r ::= rx22;;
+        tree_copy (r);;
+        y22 <-- @read ptr r;
+        y3 <-- allocb null 3;
+        r ::= y3;;
+        (y3 .+ 1) ::= y12;;
+        (y3 .+ 2) ::= y22;;
+        y3 ::= vx22;;
+        ret tt
+    )).
+Obligation Tactic := intro; move=>r; ssl_program_simpl.
+Next Obligation.
+ssl_ghostelim_pre.
+move=>[x2 s].
+ex_elim h_tree_x2s_a.
+move=>[sigma_self].
+subst.
+move=>H_tree_x2s_a.
+ssl_ghostelim_post.
+ssl_read.
+ssl_open.
+ssl_open_post H_tree_x2s_a.
+move=>[phi_tree_x2s_a].
+move=>[sigma_tree_x2s_a].
+subst.
+ssl_emp;
+exists (0);
+exists (empty);
+exists (empty);
+sslauto.
+unfold_constructor 1;
+sslauto.
+unfold_constructor 1;
+sslauto.
+ssl_open_post H_tree_x2s_a.
+ex_elim vx22 s1x2 s2x2 lx22 rx22.
+ex_elim h_tree_lx22s1x2_521x2 h_tree_rx22s2x2_522x2.
+move=>[phi_tree_x2s_a].
+move=>[sigma_tree_x2s_a].
+subst.
+move=>[H_tree_lx22s1x2_521x2 H_tree_rx22s2x2_522x2].
+ssl_read.
+ssl_read.
+ssl_read.
+ssl_write r.
+ssl_call_pre (r :-> lx22 \+ h_tree_lx22s1x2_521x2).
+ssl_call (lx22, s1x2).
+exists (h_tree_lx22s1x2_521x2);
+sslauto.
+move=>h_call3.
+ex_elim y12.
+ex_elim h_tree_lx22s1x2_521x2 h_tree_y12s1x2_521x2.
+move=>[sigma_call3].
+subst.
+move=>[H_tree_lx22s1x2_521x2 H_tree_y12s1x2_521x2].
+store_valid.
+ssl_read.
+ssl_write r.
+ssl_call_pre (r :-> rx22 \+ h_tree_rx22s2x2_522x2).
+ssl_call (rx22, s2x2).
+exists (h_tree_rx22s2x2_522x2);
+sslauto.
+move=>h_call4.
+ex_elim y22.
+ex_elim h_tree_rx22s2x2_522x2 h_tree_y22s2x2_522x2.
+move=>[sigma_call4].
+subst.
+move=>[H_tree_rx22s2x2_522x2 H_tree_y22s2x2_522x2].
+store_valid.
+ssl_read.
+ssl_alloc y3.
+ssl_write r.
+ssl_write_post r.
+ssl_write (y3 .+ 1).
+ssl_write_post (y3 .+ 1).
+ssl_write (y3 .+ 2).
+ssl_write_post (y3 .+ 2).
+ssl_write y3.
+ssl_write_post y3.
+ssl_emp;
+exists (y3);
+exists (x2 :-> vx22 \+ x2 .+ 1 :-> lx22 \+ x2 .+ 2 :-> rx22 \+ h_tree_lx22s1x2_521x2 \+ h_tree_rx22s2x2_522x2);
+exists (y3 :-> vx22 \+ y3 .+ 1 :-> y12 \+ y3 .+ 2 :-> y22 \+ h_tree_y12s1x2_521x2 \+ h_tree_y22s2x2_522x2);
+sslauto.
+unfold_constructor 2;
+exists (vx22), (s1x2), (s2x2), (lx22), (rx22);
+exists (h_tree_lx22s1x2_521x2);
+exists (h_tree_rx22s2x2_522x2);
+sslauto.
+unfold_constructor 2;
+exists (vx22), (s1x2), (s2x2), (y12), (y22);
+exists (h_tree_y12s1x2_521x2);
+exists (h_tree_y22s2x2_522x2);
+sslauto.
+
+Qed.
