examples/tree_size.v
@@ -1,0 +1,157 @@
+From mathcomp
+Require Import ssreflect ssrbool ssrnat eqtype seq ssrfun.
+From fcsl
+Require Import prelude pred pcm unionmap heap.
+From HTT
+Require Import stmod stsep stlog stlogR.
+From SSL
+Require Import core.
+
+(*
+
+predicate treeN(loc x, int n) {
+|  x == 0        => { n == 0 ; emp }
+|  not (x == 0)  => { n == 1 + n1 + n2  /\  0 <= n1  /\  0 <= n2 ;
+  [x, 3] ** x :-> v ** (x + 1) :-> l ** (x + 2) :-> r ** treeN(l, n1) ** treeN(r, n2)}
+}
+
+
+{0 <= n ; r :-> 0 ** treeN(x, n)<a> }
+void tree_size(loc x, loc r)
+{true ; r :-> n ** treeN(x, n)<a> }
+
+#####
+
+void tree_size (loc x, loc r) {
+  if (x == 0) {
+  } else {
+    let l = *(x + 1);
+    let rx = *(x + 2);
+    tree_size(l, r);
+    let n1 = *r;
+    *r = 0;
+    tree_size(rx, r);
+    let n = *r;
+    *r = 1 + n1 + n;
+  }
+}
+
+*)
+
+Inductive tree (x : ptr) (s : seq nat) (h : heap) : Prop :=
+| tree1 of x == 0 of
+  perm_eq (s) (nil) /\ h = empty
+| tree2 of ~~ (x == 0) of
+  exists (v : nat) (s1 : seq nat) (s2 : seq nat) l r,
+  exists h_tree_ls1_513 h_tree_rs2_514,
+  perm_eq (s) ([:: v] ++ s1 ++ s2) /\ h = x :-> v \+ x .+ 1 :-> l \+ x .+ 2 :-> r \+ h_tree_ls1_513 \+ h_tree_rs2_514 /\ tree l s1 h_tree_ls1_513 /\ tree r s2 h_tree_rs2_514.
+
+Inductive treeN (x : ptr) (n : nat) (h : heap) : Prop :=
+| treeN1 of x == 0 of
+  n == 0 /\ h = empty
+| treeN2 of ~~ (x == 0) of
+  exists n1 n2 l r (v: nat) (**),
+  exists h_treeN_ln1_515 h_treeN_rn2_516,
+  n == 1 + n1 + n2 /\ h = x :-> v \+ x .+ 1 :-> l \+ x .+ 2 :-> r \+ h_treeN_ln1_515 \+ h_treeN_rn2_516 /\ treeN l n1 h_treeN_ln1_515 /\ treeN r n2 h_treeN_rn2_516.
+
+Definition tree_size_type :=
+  forall (vprogs : ptr * ptr),
+  {(vghosts : nat)},
+  STsep (
+    fun h =>
+      let: (x, r) := vprogs in
+      let: (n) := vghosts in
+      exists h_treeN_xn_a,
+      0 <= n /\ h = r :-> 0 \+ h_treeN_xn_a /\ treeN x n h_treeN_xn_a,
+    [vfun (_: unit) h =>
+      let: (x, r) := vprogs in
+      let: (n) := vghosts in
+      exists h_treeN_xn_a,
+      h = r :-> n \+ h_treeN_xn_a /\ treeN x n h_treeN_xn_a
+    ]).
+Program Definition tree_size : tree_size_type :=
+  Fix (fun (tree_size : tree_size_type) vprogs =>
+    let: (x, r) := vprogs in
+    Do (
+      if x == 0
+      then
+        ret tt
+      else
+        lx2 <-- @read ptr (x .+ 1);
+        rx2 <-- @read ptr (x .+ 2);
+        tree_size (lx2, r);;
+        n1x2 <-- @read nat r;
+        r ::= 0;;
+        tree_size (rx2, r);;
+        n2x2 <-- @read nat r;
+        r ::= 1 + n1x2 + n2x2;;
+        ret tt
+    )).
+Obligation Tactic := intro; move=>[x r]; ssl_program_simpl.
+Next Obligation.
+ssl_ghostelim_pre.
+move=>n.
+ex_elim h_treeN_xn_a.
+move=>[phi_self].
+move=>[sigma_self].
+subst.
+move=>H_treeN_xn_a.
+ssl_ghostelim_post.
+ssl_open.
+ssl_open_post H_treeN_xn_a.
+move=>[phi_treeN_xn_a].
+move=>[sigma_treeN_xn_a].
+subst.
+ssl_emp;
+exists (empty);
+sslauto.
+(**)move/eqP in phi_treeN_xn_a.
+rewrite phi_treeN_xn_a=>//=.
+unfold_constructor 1;
+sslauto.
+ssl_open_post H_treeN_xn_a.
+ex_elim n1x2 n2x2 lx2 rx2 vx2.
+ex_elim h_treeN_lx2n1x2_515x h_treeN_rx2n2x2_516x.
+move=>[phi_treeN_xn_a].
+move=>[sigma_treeN_xn_a].
+subst.
+move=>[H_treeN_lx2n1x2_515x H_treeN_rx2n2x2_516x].
+ssl_read.
+ssl_read.
+ssl_call_pre (r :-> 0 \+ h_treeN_lx2n1x2_515x).
+ssl_call (n1x2).
+exists (h_treeN_lx2n1x2_515x);
+sslauto.
+move=>h_call1.
+ex_elim h_treeN_lx2n1x2_515x.
+move=>[sigma_call1].
+subst.
+move=>H_treeN_lx2n1x2_515x.
+store_valid.
+ssl_read.
+ssl_write r.
+ssl_call_pre (r :-> 0 \+ h_treeN_rx2n2x2_516x).
+ssl_call (n2x2).
+exists (h_treeN_rx2n2x2_516x);
+sslauto.
+move=>h_call2.
+ex_elim h_treeN_rx2n2x2_516x.
+move=>[sigma_call2].
+subst.
+move=>H_treeN_rx2n2x2_516x.
+store_valid.
+ssl_read.
+ssl_write r.
+ssl_write_post r.
+(**)move/eqP in phi_treeN_xn_a.
+subst.
+ssl_emp;
+exists (x :-> vx2 \+ x .+ 1 :-> lx2 \+ x .+ 2 :-> rx2 \+ h_treeN_lx2n1x2_515x \+ h_treeN_rx2n2x2_516x).
+split.
+hhauto.
+unfold_constructor 2;
+exists (n1x2), (n2x2), (lx2), (rx2), (vx2);
+exists (h_treeN_lx2n1x2_515x);
+exists (h_treeN_rx2n2x2_516x);
+sslauto.
+Qed.
