lib/core.v
@@ -19,14 +19,35 @@ Inductive ltac_No_arg : Set :=
 
 (* Utilities to move a heaplet around within a heap *)
 Ltac put_to_tail_ptr p :=
-  rewrite -?joinA; rewrite ?(joinC (p :-> _) _); rewrite ?joinA.
+  try rewrite ptrA; rewrite -?joinA; rewrite ?(joinC (p :-> _) _); rewrite ?joinA.
 
 Ltac put_to_tail h :=
-  rewrite -?joinA; rewrite ?(joinC h _); rewrite ?joinA.
+  try rewrite ptrA; rewrite -?joinA; rewrite ?(joinC h _); rewrite ?joinA.
+
+Ltac put_to_head_ptr p :=
+  put_to_tail p;
+  try rewrite (joinC _ (p :-> _)).
 
 Ltac put_to_head h :=
   put_to_tail h;
-  rewrite (joinC _ h).
+  try rewrite (joinC _ h).
+
+(* Utilities for nat and seq nat *)
+
+Ltac put_to_tail_nat n :=
+  rewrite -?addnA; rewrite ?(addnC n _); rewrite ?addnA.
+
+Ltac nat_add_eq' ns :=
+  match ns with
+  | ?A + ?B => put_to_tail_nat B; nat_add_eq' A
+  | ?A => put_to_tail A
+  end.
+
+Ltac nat_add_eq :=
+  by rewrite ?addnA;
+  match goal with
+  | [|- ?LHS = _] => nat_add_eq' LHS
+  end.
 
 (* Store heap validity assertions *)
 Ltac store_valid :=
@@ -76,15 +97,34 @@ Ltac unfold_constructor n :=
 Lemma subset_singleton :
     forall (s1: seq nat) (x: nat),
       {subset s1 <= [::x]} -> {subset x :: s1 <= [::x]}.
-intros.
-move=>n.
+Proof.
+move=>s1 x H n.
 rewrite inE; move/orP. case.
 move/eqP=>->. by rewrite inE eqxx.
 move/H=>//.
 Qed.
 
+Lemma perm_eq_nil_r: forall (A: eqType) (s: seq A), perm_eq s nil -> s = nil.
+Proof. by move=>t s; move/perm_nilP. Qed.
+
+Lemma perm_eq_nil_l: forall (A: eqType) (s: seq A), perm_eq nil s -> s = nil.
+Proof. by move=>t s; rewrite perm_sym; move/perm_nilP. Qed.
+
+Ltac seqnatauto :=
+  repeat match goal with
+  | [H: is_true (perm_eq _ nil) |- _] =>
+    apply perm_eq_nil_r in H; subst
+  | [H: is_true (perm_eq nil _) |- _] =>
+    apply perm_eq_nil_l in H; subst
+  | [|- is_true (perm_eq ?s1 ?s2)] =>
+    apply/permP=>//=?; nat_add_eq
+  | [H: {subset ?s1 <= ?s2} |- {subset _ :: ?s1 <= ?s2}] =>
+    apply: subset_singleton=>//
+  end.
+
+(* Various strategies to solve all parts of the current goal except the predicate applications  *)
 Ltac sslauto :=
-  (* Various strategies to solve all parts of the current goal except the predicate applications  *)
+  subst;
   match goal with
   | [|- verify _ _ _] => idtac
   | _ => rewrite ?unitL ?unitR;
@@ -94,13 +134,24 @@ Ltac sslauto :=
                 | [|- ?h = _] => match type of h with
                                  | (PCM.sort heapPCM) => hhauto
                                  | (PCM.sort (union_map_classPCM heapUMC)) => hhauto
-                                 | _ => auto
+                                 | _ => subst; auto
                                  end
                 | [H: is_true (_ <= _) |- _] => case: ltngtP H=>//
                 | [H: (_ <= _) = false |- _] => case: ltngtP H=>//
-                | [H: {subset ?s1 <= ?s2} |- {subset _ :: ?s1 <= ?s2}] => apply: subset_singleton=>//
+                | _ => seqnatauto
                 end
   end.
+
+Ltac ex_elim1 A := try clear dependent A; move=>[A].
+Ltac ex_elim2 A B := try clear dependent A; try clear dependent B; move=>[A][B].
+Ltac ex_elim3 A B C := try clear dependent A; try clear dependent B; try clear dependent C; move=>[A][B][C].
+
+Tactic Notation "ex_elim" ident(A) := ex_elim1 A.
+Tactic Notation "ex_elim" ident(A) ident(B) := ex_elim2 A B.
+Tactic Notation "ex_elim" ident(A) ident(B) ident(C) := ex_elim3 A B C.
+Tactic Notation "ex_elim" ident(A) ident(B) ident(C) ident(D) := ex_elim2 A B; ex_elim2 C D.
+Tactic Notation "ex_elim" ident(A) ident(B) ident(C) ident(D) ident(E) := ex_elim2 A B; ex_elim3 C D E.
+Tactic Notation "ex_elim" ident(A) ident(B) ident(C) ident(D) ident(E) ident(F) := ex_elim3 A B C; ex_elim3 D E F.
 
 (***********)
 (* Tactics *)
@@ -111,7 +162,7 @@ Ltac ssl_program_simpl := Tactics.program_simpl.
 
 
 (* Ghost Variable Elim *)
-Ltac ssl_ghostelim_pre := try apply: ghR; move=>h.
+Ltac ssl_ghostelim_pre := try apply: ghR; move=>h//=.
 
 Ltac ssl_ghostelim_post := store_valid.
 
@@ -119,7 +170,9 @@ Ltac ssl_ghostelim_post := store_valid.
 Ltac ssl_read := apply: bnd_readR=>/=.
 
 (* Write Rule *)
-Ltac ssl_write := apply: bnd_writeR=>/=.
+Ltac ssl_write x :=
+  put_to_head_ptr x; (* this significantly speeds up bnd_writeR *)
+  apply: bnd_writeR=>/=.
 
 Ltac ssl_write_post x :=
   (put_to_tail_ptr x + rewrite -(unitL (x :-> _))); apply frame.
@@ -146,7 +199,7 @@ Ltac ssl_dealloc :=
 (* Call Rule *)
 Ltac ssl_call_pre_aux h :=
   match h with
-  | ?h1 \+ ?h2 => ssl_call_pre_aux h2; put_to_head h1
+  | ?h1 \+ ?h2 => put_to_head h2; ssl_call_pre_aux h1
   | _ => put_to_head h
   end.
 
